Finish locked_AsyncRead_ok with some cleanup
Factoring out the stability proof into an alternate spec for Yield
simplifies things - the right structure is probably to have that spec
be local to the module, with the _ok prog hint unexported, so it isn't
used elsewhere, since it is specific to what is stable for this module.

More generally though it might be useful to allow instantiating Yield_ok
with a stable fact to apply to the postcondition (or automating this
pattern for the many specs that will have star R' in their
postcondition).

src/ConcurrentDisk.v
@@ -107,8 +107,9 @@ Module Type DiskSemantics (SemVars: SemanticsVars) (Sem:Semantics SemVars) (DVar
   (** Predicate asserting the relation R ignores changes to locked
   addresses in the resource r_var (a linear_mem) protected by the set
   of locks in lock_var *)
-  Definition respects_lock contents (R: ID -> Relation contents)
-             lock_var V r_var :=
+  Polymorphic Definition respects_lock contents (R: ID -> Relation contents)
+             (lock_var: member Locks.S contents) V
+             (r_var: member (@linear_mem addr (@weq _) V) contents) :=
     forall tid s s',
     forall a tid',
       Locks.get (get lock_var s) a = Owned tid' ->
@@ -285,6 +286,9 @@ Ltac simplify_reduce_step :=
           || destruct_ands
           || descend
           || subst
+          || (progress simpl_get_set)
+          (* likely a dangerous hint, partly because it applies to Learnt markers *)
+(*          || (time "autorewrite view upd *" autorewrite with view upd in * ) *)
           || invariant_unfold
           || specific_owner
           || disk_rep_unfold
@@ -343,26 +347,81 @@ Qed.
 
 (* sanity check respects_lock idea; also hides a more general proof
 that linear_rel respects the lock/resource pair it is about. *)
-Theorem diskR_respects_lock : respects_lock diskR GLocks GDisk.
+Polymorphic Theorem diskR_respects_lock : respects_lock diskR GLocks GDisk.
 Proof.
   unfold respects_lock, diskR, linear_rel, linear_upd; intuition; simpl_get_set.
   simpl_get_set in H3.
-  unfold AddrM.sz, Locks.S, Locks.A, Map.t in *.
   destruct (weq a a0); subst; try congruence.
   assert (tid' = tid'0) by congruence; subst; cleanup.
 
   erewrite H4 by eauto.
   destruct matches;
-  unfold AddrM.sz, Locks.S, Locks.A, Map.t, word_dec in *;
   autorewrite with upd; eauto;
   repeat match goal with
          | [ v: V' _ _ |- _ ] => destruct v
          end;
   repeat inv_prod;
-  congruence.
+  try congruence.
 
   destruct matches; autorewrite with upd; eauto.
 Qed.
+
+(* prove for one step first *)
+Lemma locked_addr_stable' : forall tid a s s',
+    (view Latest (get GDisk s) a = view Latest (get GDisk s) a /\
+     Locks.get (get GLocks s) a = Owned tid) ->
+    othersR R tid s s' ->
+    view Latest (get GDisk s') a =
+    view Latest (get GDisk s) a /\
+    Locks.get (get GLocks s') a = Owned tid.
+Proof.
+  intros; destruct_ands.
+  apply others_disk_relation_holds in H0.
+  unfold othersR, diskR, view, linear_rel in *; deex;
+  specialize_all Locks.A.
+  - erewrite H5; eauto.
+  - inversion H3; subst; congruence.
+Qed.
+
+Lemma locked_addr_stable {s s' tid a} :
+  Locks.get (get GLocks s) a = Owned tid ->
+  star (othersR R tid) s s' ->
+  view Latest (get GDisk s') a =
+  view Latest (get GDisk s) a /\
+  Locks.get (get GLocks s') a = Owned tid.
+Proof.
+  intros.
+  apply (star_invariant _ _ (@locked_addr_stable' tid a));
+    intuition (eauto || congruence).
+Qed.
+
+Definition locked_yield {T} a rx : prog Mcontents Scontents T :=
+  Yield a;;
+        rx tt.
+
+Polymorphic Theorem locked_yield_ok : forall a,
+  stateS TID: tid |-
+  {{ v,
+   | PRE d m s0 s:
+       Inv m s d /\
+       Locks.get (get GLocks s) a = Owned tid /\
+       view Latest (get GDisk s) a = v /\
+       R tid s0 s
+   | POST d' m' s0' s' _:
+         Inv m' s' d' /\
+         star (othersR R tid) s s' /\
+         Locks.get (get GLocks s') a = Owned tid /\
+         view Latest (get GDisk s') a = v /\
+         R tid s0' s'
+  }} locked_yield a.
+Proof.
+  hoare pre simplify with try solve [ finish ].
+  eapply locked_addr_stable; eauto.
+  eapply locked_addr_stable; eauto.
+  apply R_trans; eauto.
+Qed.
+
+Hint Extern 1 {{ locked_yield _; _ }} => apply locked_yield_ok : prog.
 
 Definition locked_AsyncRead {T} a rx : prog Mcontents Scontents T :=
   tid <- GetTID;
@@ -376,7 +435,7 @@ Definition locked_AsyncRead {T} a rx : prog Mcontents Scontents T :=
                             end in
                  (set GDisk vd' s));;
               StartRead_upd a;;
-              Yield a;;
+              locked_yield a;;
               v <- FinishRead_upd a;
   GhostUpdate (fun s =>
                  let vd := get GDisk s in
@@ -427,51 +486,15 @@ Proof.
   eapply view_lift_upd; eauto.
 Qed.
 
-Hint Rewrite view_hide_upd : view.
-Hint Rewrite view_lift_upd_hint using (now eauto) : view.
+Polymorphic Hint Rewrite view_hide_upd : view.
+Polymorphic Hint Rewrite view_lift_upd_hint using (now eauto) : view.
+
+(*
 (* the above hints don't fire when the below does, for some reason
 (probably related to universes) *)
 Hint Rewrite (@view_hide_upd addr _ (const wr_set)) : view.
 Hint Rewrite (@view_lift_upd_hint addr _ (const wr_set)) using (now eauto) : view.
-
-(* prove for one step first *)
-Lemma locked_addr_stable' : forall tid a s s',
-    (view Latest (get GDisk s) a = view Latest (get GDisk s) a /\
-     Locks.get (get GLocks s) a = Owned tid) ->
-    othersR R tid s s' ->
-    view Latest (get GDisk s') a =
-    view Latest (get GDisk s) a /\
-    Locks.get (get GLocks s') a = Owned tid.
-Proof.
-  intros; destruct_ands.
-  apply others_disk_relation_holds in H0.
-  unfold othersR, diskR, view, linear_rel in *; deex;
-  specialize_all Locks.A.
-  - erewrite H5; eauto.
-  - inversion H3; subst; congruence.
-Qed.
-
-Lemma simple_star_invariant : forall A (P: A -> Prop) (R: relation A),
-    (forall s s', P s -> R s s' -> P s') ->
-    (forall s s', P s -> star R s s' -> P s').
-Proof.
-  intros.
-  induction H1; eauto.
-Qed.
-
-Lemma locked_addr_stable {s s' tid a} :
-  Locks.get (get GLocks s) a = Owned tid ->
-  star (othersR R tid) s s' ->
-  view Latest (get GDisk s') a =
-  view Latest (get GDisk s) a /\
-  Locks.get (get GLocks s') a = Owned tid.
-Proof.
-  intros.
-  apply (star_invariant _ _ (@locked_addr_stable' tid a)); intuition (eauto || congruence).
-Qed.
-
-Hint Immediate linear_rel_refl.
-
+*)
 
 Polymorphic Theorem respects_lock_others' : forall tid s s' a,
     Locks.get (get GLocks s) a = Owned tid ->
@@ -486,7 +509,6 @@ Proof.
   eexists; intuition eauto.
   eapply relation_respects_lock; eauto.
 
-  Search diskR.
   apply disk_relation_holds in H2.
   unfold diskR, linear_rel in H2; intuition.
   specialize_all Locks.A.
@@ -507,8 +529,7 @@ Proof.
   intuition eauto.
 Qed.
 
-(** TODO: move these two lemmas to Linearizable, add to a linear_upd
-Rewrite HintDb similar to upd *)
+(** TODO: move these two lemmas to Linearizable *)
 Polymorphic Lemma linear_upd_repeat : forall A AEQ V (m: @linear_mem A AEQ V) a v v',
     linear_upd (linear_upd m a v) a v' = linear_upd m a v'.
 Proof.
@@ -530,6 +551,11 @@ Proof.
   cbn in *;
   try congruence.
 Qed.
+
+Polymorphic Hint Rewrite linear_upd_repeat : linear_upd.
+Polymorphic Hint Rewrite linear_upd_same using (solve [ auto ]) : linear_upd.
+
+Hint Resolve linear_rel_refl.
 
 Polymorphic Theorem locked_AsyncRead_ok : forall a,
   stateS TID: tid |-
@@ -553,84 +579,56 @@ Proof.
   step pre simplify with try solve [ finish ].
   step pre simplify with try solve [ finish ].
   step pre simplify with try solve [ finish ].
-
   step pre simplify with try solve [ finish ].
-  unfold pred_in.
-  finish.
 
-  unfold diskI; intuition; simpl_get_set;
-  autorewrite with view; auto.
+  finish.
+  unfold diskI; simplify; autorewrite with view; eauto.
   eapply linearized_consistent_upd; eauto.
 
   apply R_trans.
   eapply star_two_step; eauto.
   finish.
-  unfold diskR; intuition; simpl_get_set.
+  unfold diskR; simplify.
   (* BUG: eauto using linear_rel_upd gives exception
   Univ.AlreadyDeclared *)
   eapply linear_rel_upd; eauto.
 
   step pre simplify with try solve [ finish ].
-  unfold pred_in in *.
-  simplify; eauto.
-
-  unfold StateR' in *.
-  match goal with
-  | [ H: star (othersR R tid) ?s ?s', a: addr |- _ ] =>
-    let Hl := fresh in
-    assert (Locks.get (get GLocks s) a = Owned tid) as Hl by simpl_get_set;
-      learn that (locked_addr_stable Hl H);
-      clear Hl
-  end; destruct_ands.
-
-  rewrite H14.
-  simpl_get_set.
-  autorewrite with view upd.
+  autorewrite with upd view in *.
   eauto.
 
   step pre simplify with try solve [ finish ].
-  step pre simplify with try solve [ finish ].
+  step pre simplify with try solve [ finish ];
+    autorewrite with upd view in *;
+    simplify.
 
-  unfold pred_in in *; simplify.
   finish.
-  (* same as locked stable proof above *)
-  assert (view Latest (get GDisk s2) a = Some (v, Some tid)) by admit.
-  simpl_match.
-  unfold diskI; intuition; simpl_get_set;
-  autorewrite with view; eauto.
+  unfold diskI; intuition;
+    repeat (autorewrite with upd view in * || simplify);
+    eauto.
   eapply linearized_consistent_upd; eauto.
-  admit. (* using locked_addr_stable would have given this as well *)
 
-  simpl_get_set.
-  assert (view Latest (get GDisk s2) a = Some (v, Some tid)) by admit.
-  simpl_match.
-  autorewrite with view upd; auto.
+  autorewrite with upd view; auto.
 
-  unfold StateR' in *.
-  assert (view Latest (get GDisk s2) a = Some (v, Some tid)) by admit.
-  simpl_match.
+  match goal with
+  | [ H: star (othersR R tid) _ _ |- _ ] =>
+    eapply respects_lock_others with (v' := (v, None)) in H; simpl_get_set; eauto;
+    simpl_get_set in H;
+    autorewrite with linear_upd in H;
+    simpl_get_set in H
+  end.
 
-  eapply respects_lock_others with (v' := (v, None)) in H11; simpl_get_set; eauto.
-  simpl_get_set in H11.
-
-  rewrite linear_upd_repeat in H11.
-  rewrite linear_upd_same in H11 by eauto.
-  simpl_get_set in H11.
-
+  eapply R_trans.
+  eapply star_two_step; eauto.
   finish.
-  unfold pred_in in *.
-  simplify.
   (* BUG: can't use eauto on any generated goals due to
   Univ.AlreadyDeclared *)
   unfold diskR; simpl_get_set.
   split.
   apply same_domain_refl.
-  assert (view Latest (get GDisk s2) a = Some (v, Some tid)) by admit.
-  simpl_match.
   eapply linear_rel_upd.
-  admit.
+  auto.
   apply linear_rel_refl.
-
-Admitted.
+Qed.
 
 End LockedDisk.
